add linear pointers

concurrency/framework/Ptrs.s.dfy
@@ -2,6 +2,9 @@ module Ptrs {
   // Non-atomic memory
 
   datatype PointsTo<V> = PointsTo(ghost ptr: Ptr, ghost v: V)
+  datatype PointsToLinear<V> =
+    | PointsToLinear(ghost ptr: Ptr, ghost v: V)
+    | PointsToEmpty(ghost ptr: Ptr)
   datatype PointsToArray<V> = PointsToArray(ghost ptr: Ptr, ghost s: seq<V>)
 
   type {:extern} Ptr(!new,==)
@@ -15,6 +18,24 @@ module Ptrs {
     returns (v: V)
     requires d.ptr == this
     ensures v == d.v
+
+    method {:extern} write_linear<V>(glinear inout d: PointsToLinear<V>, linear v: V)
+    requires old_d.PointsToEmpty?
+    requires old_d.ptr == this
+    ensures d.PointsToLinear? && d.ptr == this && d.v == v
+
+    method {:extern} read_linear<V>(glinear inout d: PointsToLinear<V>)
+    returns (linear v: V)
+    requires old_d.PointsToLinear?
+    requires old_d.ptr == this
+    ensures v == old_d.v
+    ensures d.PointsToEmpty? && d.ptr == this
+
+    method {:extern} read_shared<V>(gshared d: PointsToLinear<V>)
+    returns (shared v: V)
+    requires d.PointsToLinear?
+    requires d.ptr == this
+    ensures v == old_d.v
 
     method {:extern} index_write<V>(glinear inout d: PointsToArray, i: int, v: V)
     requires old_d.ptr == this
@@ -33,4 +54,8 @@ module Ptrs {
   method {:extern} alloc<V>(v: V)
   returns (ptr: Ptr, glinear d: PointsTo<V>)
   ensures d == PointsTo(ptr, v)
+
+  method {:extern} alloc_linear<V>(linear v: V)
+  returns (ptr: Ptr, glinear d: PointsToLinear<V>)
+  ensures d == PointsToLinear(ptr, v)
 }
